\documentclass{article}
\usepackage[utf8]{inputenc}
\usepackage[T1]{fontenc}
\usepackage{amsmath}

\begin{document}
\begin{equation}
S(x) = 
   \begin{cases}
      e^{-\frac{a(t-t_0)^2}{2}} + \int_{t_0}^t a(x - t_0)e^{-\frac{a(x-t_0)^2}{2}}\cdot e^{-\lambda (t-x)}\,\mathrm{d}x & \quad \text{if } t > t_0\\
      1 & \quad \text{if } t \leq t_0
   \end{cases}
\end{equation}
\begin{equation}
S(x) = \prod_{i=1}^x (1-B_i) + \sum_{i=1}^x B_i \cdot e^{(i-x-1)\cdot r} \cdot \prod_{j=1}^{i-1} (1-B_j)
\end{equation}

\[ B_x = 
   \begin{cases}
      0 & \quad \text{if } x < t_0 = -\frac{b}{a}\\
      1 - e^{-ax + at_0 + a/2} & \quad \text{if } x \geq t_0\\
%      ax + b & \quad \text{if } -\frac{b}{a} \leq x \leq \frac{1-b}{a}\\
%      1 & \quad \text{if } x > \frac{1-b}{a} = t_1
   \end{cases}
\]

\begin{equation}
S(x) = \prod_{i>t_0}^x e^{-ai+at_0+a/2} + \sum_{i>t_0}^x (1-e^{-ai+at_0+a/2})\cdot e^{(i-x-1)r} \cdot \prod_{j>t_0}^{i-1}e^{-aj+at_0+a/2}
\end{equation}

\end{document}
